\documentclass[../cheatSheetAlgoritmi.tex]{subfiles}
\begin{document}

\section{Regole Matematiche} \subsection{Sommatorie}
\textbf{Serie Geometrica Finita}: $\forall$$x \neq 1 : \sum\limits_{j=0}^{k} {x^{j}}$ = $\frac{x^{k+1} - 1}{x - 1}$ \\
\textbf{Serie Geometrica Infinita Decrescente}: $\forall$x, $\mid x \mid$ $<$ $1$ : $\sum\limits_{i=0}^{\infty} {x^{i}}$ = ${\frac{1}{1-x}}$
\subsection{Cambiamento di Base}
$\log_{b}{n} = (\log_{b}{a})(\log_{a}{n}) \implies a^{\log_{b}{n}} = n^{\log_{b}{a}}$

\newpage
\end{document}